alternative machine interface specification proposal

src/BoundedArithmetic/ArchitectureToZLike.v
@@ -3,6 +3,8 @@ Require Import Coq.ZArith.ZArith.
 Require Import Crypto.BoundedArithmetic.Interface.
 Require Import Crypto.BoundedArithmetic.DoubleBounded.
 Require Import Crypto.ModularArithmetic.ZBounded.
+Require Import Coq.Lists.List.
+Import ListNotations.
 
 Local Open Scope nat_scope.
 Local Open Scope Z_scope.
@@ -10,13 +12,97 @@ Local Open Scope type_scope.
 
 Local Coercion Z.of_nat : nat >-> Z.
 
-Local Existing Instances DoubleArchitectureBoundedOps DoubleArchitectureBoundedFullMulOpsOfHalfWidthMulOps DoubleArchitectureBoundedHalfWidthMulOpsOfFullMulOps.
-
-Section ops.
+Section fancy_machine_p256_montgomery_foundation.
   Context {n_over_two : size}.
   Local Notation n := (2 * n_over_two)%nat.
-  Context (ops : ArchitectureBoundedOps n) (mops : ArchitectureBoundedHalfWidthMulOps n)
-          (modulus : Z).
+  Context (ops : fancy_machine.instructions n) (modulus : Z).
+
+  Definition two_list_to_tuple {A B} (x : A * list B)
+    := match x return match x with
+                      | (a, [b0; b1]) => A * (B * B)
+                      | _ => True
+                      end
+       with
+       | (a, [b0; b1]) => (a, (b0, b1))
+       | _ => I
+       end.
+
+  (* make all machine-specific constructions here, preferrably as
+  thing wrappers around generic constructions *)
+    Local Instance DoubleArchitectureBoundedOps : ArchitectureBoundedOps (2 * n)%nat
+      := { BoundedType := BoundedType * BoundedType (* [(high, low)] *);
+           decode high_low := (decode (fst high_low) * 2^n + decode (snd high_low))%Z;
+           encode z := (encode (z / 2^n), encode (z mod 2^n));
+           ShiftRight a high_low
+           := let '(high, low) := eta high_low in
+              if n <=? a then
+                (ShiftRight (a - n)%nat (encode 0, fst high), ShiftRight (a - n)%nat high)
+              else
+                (ShiftRight a (snd high, fst low), ShiftRight a low);
+           ShiftLeft a high_low
+           := let '(high, low) := eta high_low in
+              if 2 * n <=? a then
+                let '(high0, low) := eta (ShiftLeft (a - 2 * n)%nat low) in
+                let '(high_high, high1) := eta (ShiftLeft (a - 2 * n)%nat high) in
+                ((snd (CarryAdd false high0 high1), low), (encode 0, encode 0))
+              else if n <=? a then
+                     let '(high0, low) := eta (ShiftLeft (a - n)%nat low) in
+                     let '(high_high, high1) := eta (ShiftLeft (a - n)%nat high) in
+                     ((high_high, snd (CarryAdd false high0 high1)), (low, encode 0))
+                   else
+                     let '(high0, low) := eta (ShiftLeft a low) in
+                     let '(high_high, high1) := eta (ShiftLeft a high) in
+                     ((encode 0, high_high), (snd (CarryAdd false high0 high1), low));
+           Mod2Pow a high_low
+           := let '(high, low) := (fst high_low, snd high_low) in
+              (Mod2Pow (a - n)%nat high, Mod2Pow a low);
+           CarryAdd carry x_high_low y_high_low
+           := let '(xhigh, xlow) := eta x_high_low in
+              let '(yhigh, ylow) := eta y_high_low in
+              two_list_to_tuple (ripple_carry CarryAdd carry [xhigh; xlow] [yhigh; ylow]);
+           CarrySub carry x_high_low y_high_low
+           := let '(xhigh, xlow) := eta x_high_low in
+              let '(yhigh, ylow) := eta y_high_low in
+              two_list_to_tuple (ripple_carry CarrySub carry [xhigh; xlow] [yhigh; ylow]) }.
+
+    Definition BoundedOfHalfBounded (x : @BoundedHalfType (2 * n)%nat _) : @BoundedType n _
+      := match x with
+         | UpperHalf x => fst x
+         | LowerHalf x => snd x
+         end.
+
+    Local Instance DoubleArchitectureBoundedHalfWidthMulOpsOfFullMulOps
+          {base_mops : ArchitectureBoundedFullMulOps n}
+      : ArchitectureBoundedHalfWidthMulOps (2 * n)%nat :=
+      { HalfWidthMul a b
+        := Mul (BoundedOfHalfBounded a) (BoundedOfHalfBounded b) }.
+  End single.
+
+  Local Existing Instance DoubleArchitectureBoundedOps.
+
+  Section full_from_half.
+    Context (n : size) {base_ops : ArchitectureBoundedOps (2 * n)%nat}.
+
+    Local Infix "*" := HalfWidthMul.
+
+    Local Instance DoubleArchitectureBoundedFullMulOpsOfHalfWidthMulOps
+          {base_mops : ArchitectureBoundedHalfWidthMulOps (2 * n)%nat}
+      : ArchitectureBoundedFullMulOps (2 * n)%nat :=
+      { Mul a b
+        := let '(a1, a0) := (UpperHalf a, LowerHalf a) in
+           let '(b1, b0) := (UpperHalf b, LowerHalf b) in
+           let out := a0 * b0 in
+           let outHigh := a1 * b1 in
+           let tmp := a1 * b0 in
+           let '(carry, out) := eta (CarryAdd false out (snd (ShiftLeft n tmp))) in
+           let '(_, outHigh) := eta (CarryAdd carry outHigh (ShiftRight n (encode 0, tmp))) in
+           let tmp := a0 * b1 in
+           let '(carry, out) := eta (CarryAdd false out (snd (ShiftLeft n tmp))) in
+           let '(_, outHigh) := eta (CarryAdd carry outHigh (ShiftRight n (encode 0, tmp))) in
+           (outHigh, out) }.
+  End full_from_half.
+
+  Local Existing Instance DoubleArchitectureBoundedFullMulOpsOfHalfWidthMulOps.
 
   Axiom admit : forall {T}, T.
 
@@ -36,3 +122,5 @@ Section ops.
       ConditionalSubtract b x := admit;
       ConditionalSubtractModulus y := admit }.
 End ops.
+
+End with_single_ops.
