src/BoundedArithmetic/DoubleBounded.v
@@ -13,102 +13,18 @@ Local Open Scope type_scope.
 Local Coercion Z.of_nat : nat >-> Z.
 Local Notation eta x := (fst x, snd x).
 
-Section with_single_ops.
-  Section single.
-    Context (n : size) {base_ops : ArchitectureBoundedOps n}.
+Section generic_constructions.
+  Definition ripple_carry {T} (f : T -> T -> bool -> bool * T)
+             (carry : bool) (xs ys : list T) : bool * list T
+    := List.fold_right
+         (fun x_y carry_zs => let '(x, y) := eta x_y in
+                              let '(carry, zs) := eta carry_zs in
+                              let '(carry, z) := eta (f x y carry) in
+                              (carry, z :: zs))
+         (carry, nil)
+         (List.combine xs ys).
 
-    Definition ripple_carry {T} (f : bool -> T -> T -> bool * T)
-               (carry : bool) (xs ys : list T) : bool * list T
-      := List.fold_right
-           (fun x_y carry_zs => let '(x, y) := eta x_y in
-                                let '(carry, zs) := eta carry_zs in
-                                let '(carry, z) := eta (f carry x y) in
-                                (carry, z :: zs))
-           (carry, nil)
-           (List.combine xs ys).
+  (* TODO: Would it made sense to make generic-width shift operations here? *)
 
-    Definition two_list_to_tuple {A B} (x : A * list B)
-      := match x return match x with
-                        | (a, [b0; b1]) => A * (B * B)
-                        | _ => True
-                        end
-         with
-         | (a, [b0; b1]) => (a, (b0, b1))
-         | _ => I
-         end.
-
-    Local Instance DoubleArchitectureBoundedOps : ArchitectureBoundedOps (2 * n)%nat
-      := { BoundedType := BoundedType * BoundedType (* [(high, low)] *);
-           decode high_low := (decode (fst high_low) * 2^n + decode (snd high_low))%Z;
-           encode z := (encode (z / 2^n), encode (z mod 2^n));
-           ShiftRight a high_low
-           := let '(high, low) := eta high_low in
-              if n <=? a then
-                (ShiftRight (a - n)%nat (encode 0, fst high), ShiftRight (a - n)%nat high)
-              else
-                (ShiftRight a (snd high, fst low), ShiftRight a low);
-           ShiftLeft a high_low
-           := let '(high, low) := eta high_low in
-              if 2 * n <=? a then
-                let '(high0, low) := eta (ShiftLeft (a - 2 * n)%nat low) in
-                let '(high_high, high1) := eta (ShiftLeft (a - 2 * n)%nat high) in
-                ((snd (CarryAdd false high0 high1), low), (encode 0, encode 0))
-              else if n <=? a then
-                     let '(high0, low) := eta (ShiftLeft (a - n)%nat low) in
-                     let '(high_high, high1) := eta (ShiftLeft (a - n)%nat high) in
-                     ((high_high, snd (CarryAdd false high0 high1)), (low, encode 0))
-                   else
-                     let '(high0, low) := eta (ShiftLeft a low) in
-                     let '(high_high, high1) := eta (ShiftLeft a high) in
-                     ((encode 0, high_high), (snd (CarryAdd false high0 high1), low));
-           Mod2Pow a high_low
-           := let '(high, low) := (fst high_low, snd high_low) in
-              (Mod2Pow (a - n)%nat high, Mod2Pow a low);
-           CarryAdd carry x_high_low y_high_low
-           := let '(xhigh, xlow) := eta x_high_low in
-              let '(yhigh, ylow) := eta y_high_low in
-              two_list_to_tuple (ripple_carry CarryAdd carry [xhigh; xlow] [yhigh; ylow]);
-           CarrySub carry x_high_low y_high_low
-           := let '(xhigh, xlow) := eta x_high_low in
-              let '(yhigh, ylow) := eta y_high_low in
-              two_list_to_tuple (ripple_carry CarrySub carry [xhigh; xlow] [yhigh; ylow]) }.
-
-    Definition BoundedOfHalfBounded (x : @BoundedHalfType (2 * n)%nat _) : @BoundedType n _
-      := match x with
-         | UpperHalf x => fst x
-         | LowerHalf x => snd x
-         end.
-
-    Local Instance DoubleArchitectureBoundedHalfWidthMulOpsOfFullMulOps
-          {base_mops : ArchitectureBoundedFullMulOps n}
-      : ArchitectureBoundedHalfWidthMulOps (2 * n)%nat :=
-      { HalfWidthMul a b
-        := Mul (BoundedOfHalfBounded a) (BoundedOfHalfBounded b) }.
-  End single.
-
-  Local Existing Instance DoubleArchitectureBoundedOps.
-
-  Section full_from_half.
-    Context (n : size) {base_ops : ArchitectureBoundedOps (2 * n)%nat}.
-
-    Local Infix "*" := HalfWidthMul.
-
-    Local Instance DoubleArchitectureBoundedFullMulOpsOfHalfWidthMulOps
-          {base_mops : ArchitectureBoundedHalfWidthMulOps (2 * n)%nat}
-      : ArchitectureBoundedFullMulOps (2 * n)%nat :=
-      { Mul a b
-        := let '(a1, a0) := (UpperHalf a, LowerHalf a) in
-           let '(b1, b0) := (UpperHalf b, LowerHalf b) in
-           let out := a0 * b0 in
-           let outHigh := a1 * b1 in
-           let tmp := a1 * b0 in
-           let '(carry, out) := eta (CarryAdd false out (snd (ShiftLeft n tmp))) in
-           let '(_, outHigh) := eta (CarryAdd carry outHigh (ShiftRight n (encode 0, tmp))) in
-           let tmp := a0 * b1 in
-           let '(carry, out) := eta (CarryAdd false out (snd (ShiftLeft n tmp))) in
-           let '(_, outHigh) := eta (CarryAdd carry outHigh (ShiftRight n (encode 0, tmp))) in
-           (outHigh, out) }.
-  End full_from_half.
-
-  Local Existing Instance DoubleArchitectureBoundedFullMulOpsOfHalfWidthMulOps.
-End with_single_ops.
+  (* FUTURE: here go proofs about [ripple_carry] with [f] that satisfies [is_add_with_carry] *)
+End generic_constructions.
